more work on fa2token

execution/theories/Examples/FA2Interface.v
@@ -10,6 +10,7 @@ Require Import Containers.
 From RecordUpdate Require Import RecordUpdate.
 Import RecordSetNotations.
 
+Section FA2Interface.
 Context {BaseTypes : ChainBase}.
 Set Primitive Projections.
 Set Nonrecursive Elimination Schemes.
@@ -17,11 +18,12 @@ Section FA2Types.
 
 Definition token_id := N.
 
-Record callback (A : Type) := {
-  callback_addr : Address;
-  body : A;
-}.
+(* Definition callback (A : Type) := A -> ActionBody.  *)
 
+
+Record callback (A : Type) := {
+  (* callback_addr : Address; *)
+}.
 
 Record transfer :=
   build_transfer {
@@ -149,11 +151,18 @@ Inductive fa2_token_receiver :=
 Inductive fa2_token_sender :=
   | tokens_sent : transfer_descriptor_param -> fa2_token_sender.
 
+Record set_hook_param := {
+  hook : callback transfer_descriptor_param;
+  hook_permissions_descriptor : permissions_descriptor;
+}.
+
+
 End FA2Types.
+
 Section Setters.
 
-Instance callback_settable {A : Type} : Settable (callback A) :=
-  settable! (Build_callback A) <(callback_addr A); (body A)>.
+(* Instance callback_settable {A : Type} : Settable (callback A) :=
+  settable! (Build_callback A) <(callback_addr A); (body A)>. *)
   
 Instance transfer_settable : Settable transfer :=
   settable! build_transfer <from_; to_; transfer_token_id; amount>.
@@ -204,19 +213,27 @@ Instance transfer_descriptor_settable : Settable transfer_descriptor :=
 Instance transfer_descriptor_param_settable : Settable transfer_descriptor_param :=
   settable! Build_transfer_descriptor_param <transfer_descr_fa2; transfer_descr_batch; transfer_descr_operator>.
 
+Instance set_hook_param_settable : Settable set_hook_param :=
+  settable! Build_set_hook_param <hook; hook_permissions_descriptor>.
+
 End Setters.
 
 Section Serialization.
 
-(* Global Program Instance callback_serializable {A : Type} `{Serializable A} : Serializable (callback A) :=
-  {| serialize c := let addr := c.(callback_addr A) in
-                    let body := c.(body A) in
-                    serialize (addr, body);
+Global Program Instance callback_serializable {A : Type} : Serializable (callback A) :=
+  {| serialize c := @serialize unit _ tt;
      deserialize p := 
-     do prod <- @deserialize_product Address _ A _ p ;
-     Some (Build_callback A (fst prod) (snd prod)) ;
+     do tt <- @deserialize unit _ p ;
+     Some (Build_callback A)
   |}.
-Next Obligation. *)
+Next Obligation.
+intros.
+cbn.
+rewrite deserialize_serialize. 
+destruct x.
+reflexivity. 
+Qed.
+
 
 Global Instance transfer_serializable : Serializable transfer :=
   Derive Serializable transfer_rect <build_transfer>.
@@ -227,8 +244,8 @@ Global Instance balance_of_request_serializable : Serializable balance_of_reques
 Global Instance balance_of_response_serializable : Serializable balance_of_response :=
   Derive Serializable balance_of_response_rect <Build_balance_of_response>.
 
-Instance bal_of_param_callback_serializable : Serializable (callback (list balance_of_response)) :=
-  Derive Serializable (callback_rect (list balance_of_response)) <(Build_callback (list balance_of_response))>.
+(* Instance bal_of_param_callback_serializable : Serializable (callback (list balance_of_response)) :=
+  Derive Serializable (callback_rect (list balance_of_response)) <(Build_callback (list balance_of_response))>. *)
 
 Global Instance balance_of_param_serializable : Serializable balance_of_param :=
   Derive Serializable balance_of_param_rect <Build_balance_of_param>.
@@ -236,8 +253,8 @@ Global Instance balance_of_param_serializable : Serializable balance_of_param :=
 Global Instance total_supply_response_serializable : Serializable total_supply_response :=
   Derive Serializable total_supply_response_rect <Build_total_supply_response>.
 
-Instance supply_param_callback_serializable : Serializable (callback (list total_supply_response)) :=
-  Derive Serializable (callback_rect (list total_supply_response)) <(Build_callback (list total_supply_response))>.
+(* Instance supply_param_callback_serializable : Serializable (callback (list total_supply_response)) :=
+  Derive Serializable (callback_rect (list total_supply_response)) <(Build_callback (list total_supply_response))>. *)
 
 Global Instance total_supply_param_serializable : Serializable total_supply_param :=
   Derive Serializable total_supply_param_rect <Build_total_supply_param>.
@@ -245,8 +262,8 @@ Global Instance total_supply_param_serializable : Serializable total_supply_para
 Global Instance token_metadata_serializable : Serializable token_metadata :=
   Derive Serializable token_metadata_rect <Build_token_metadata>.
 
-Instance metadata_callback_serializable : Serializable (callback (list token_metadata)) :=
-  Derive Serializable (callback_rect (list token_metadata)) <(Build_callback (list token_metadata))>.
+(* Instance metadata_callback_serializable : Serializable (callback (list token_metadata)) :=
+  Derive Serializable (callback_rect (list token_metadata)) <(Build_callback (list token_metadata))>. *)
 
 Global Instance token_metadata_param_serializable : Serializable token_metadata_param :=
   Derive Serializable token_metadata_param_rect <Build_token_metadata_param>.
@@ -263,8 +280,8 @@ Global Instance update_operator_serializable : Serializable update_operator :=
 Global Instance is_operator_response_serializable : Serializable is_operator_response :=
   Derive Serializable is_operator_response_rect <Build_is_operator_response>.
 
-Instance is_operator_param_callback_serializable : Serializable (callback is_operator_response) :=
-  Derive Serializable (callback_rect is_operator_response) <(Build_callback is_operator_response)>.
+(* Instance is_operator_param_callback_serializable : Serializable (callback is_operator_response) :=
+  Derive Serializable (callback_rect is_operator_response) <(Build_callback is_operator_response)>. *)
 
 Global Instance is_operator_param_serializable : Serializable is_operator_param :=
   Derive Serializable is_operator_param_rect <Build_is_operator_param>.
@@ -296,4 +313,12 @@ Global Instance fa2_token_receiver_serializable : Serializable fa2_token_receive
 Global Instance fa2_token_sender_serializable : Serializable fa2_token_sender :=
   Derive Serializable fa2_token_sender_rect <tokens_sent>.
 
+(* Instance transfer_descriptor_param_callback_serializable : Serializable (callback transfer_descriptor_param) :=
+  Derive Serializable (callback_rect transfer_descriptor_param) <(Build_callback transfer_descriptor_param)>. *)
+
+Global Instance set_hook_param_serializable : Serializable set_hook_param :=
+  Derive Serializable set_hook_param_rect <Build_set_hook_param>.
+
 End Serialization.
+
+End FA2Interface.
