execution/theories/Examples/FA2Token.v
@@ -1,29 +1,34 @@
 From Coq Require Import ZArith.
-(* From Coq Require Import Morphisms. *)
+From Coq Require Import Morphisms.
 Require Import Monads.
 Require Import Extras.
 Require Import Containers.
-(* Require Import Automation. *)
+Require Import Automation.
 From RecordUpdate Require Import RecordUpdate.
 From Coq Require Import List.
 Require Import Serializable.
 Require Import Blockchain.
 Import ListNotations.
 Import RecordSetNotations.
+From Coq Require Import Program.Basics.
+Notation "f 'o' g" := (compose f g) (at level 50).
+
+Require Import FA2Interface. 
 
 Section FA2Token.
 Context {BaseTypes : ChainBase}.
-Require Import FA2Interface. 
 Set Primitive Projections.
 Set Nonrecursive Elimination Schemes.
 Open Scope N_scope.
 
+
 Inductive Msg := 
   | msg_transfer : list transfer -> Msg
+  | msg_set_transfer_hook : set_hook_param -> Msg
   | msg_balance_of : balance_of_param -> Msg
   | msg_total_supply : total_supply_param -> Msg
   | msg_token_metadata : token_metadata_param -> Msg
-  | msg_permissions_descriptor : permissions_descriptor -> Msg (* TODO fix callback type *)
+  | msg_permissions_descriptor : callback permissions_descriptor -> Msg (* TODO fix callback type *)
   | msg_update_operators : list update_operator -> Msg
   | msg_is_operator : is_operator_param -> Msg.
 
@@ -35,20 +40,23 @@ Record TokenLedger :=
 
 Record State :=
   build_state {
-    assets: FMap token_id TokenLedger 
+    assets            : FMap token_id TokenLedger; 
+    operators         : FMap Address (FMap Address operator_tokens);
+    permission_policy : permissions_descriptor;
   }.
 
 Record Setup :=
   build_setup {
-    setup_total_supply : list (token_id * N);
+    setup_total_supply : list (token_id * N); (* is this necessary? *)
+    permission_policy_ : permissions_descriptor;
   }.
 
 Instance token_ledger_settable : Settable _ :=
   settable! build_token_ledger <fungible; balances>.
 Instance state_settable : Settable _ :=
-  settable! build_state <assets>.
+  settable! build_state <assets; operators; permission_policy>.
 Instance setup_settable : Settable _ :=
-  settable! build_setup <setup_total_supply>.
+  settable! build_setup <setup_total_supply; permission_policy_>.
 
 Section Serialization.
 
@@ -56,7 +64,7 @@ Global Instance setup_serializable : Serializable Setup :=
   Derive Serializable Setup_rect <build_setup>.
 
 Global Instance msg_serializable : Serializable Msg :=
-  Derive Serializable Msg_rect <msg_transfer, msg_balance_of, msg_total_supply, msg_token_metadata, msg_permissions_descriptor, msg_update_operators, msg_is_operator>.
+  Derive Serializable Msg_rect <msg_transfer, msg_set_transfer_hook, msg_balance_of, msg_total_supply, msg_token_metadata, msg_permissions_descriptor, msg_update_operators, msg_is_operator>.
 
 Global Instance TokenLedger_serializable : Serializable TokenLedger :=
   Derive Serializable TokenLedger_rect <build_token_ledger>.
@@ -65,6 +73,14 @@ Global Instance state_serializable : Serializable State :=
 	Derive Serializable State_rect <build_state>.
 	
 End Serialization.
+
+(* Definition build_callback_act {A : Type} 
+                             `{Serializable A}
+                             `{Serializable (callback A)}
+                              (contract_addr : Address)
+                              (cb : callback A)
+                              : Action :=
+  build_act contract_addr (act_call cb.(callback_addr A) 0%Z (@serialize A _ cb.(body A))). *)
 
 Definition returnIf (cond : bool) := if cond then None else Some tt.
 
@@ -86,20 +102,191 @@ Definition address_has_transfer_permission (caller owner : Address) : option uni
 
 Definition address_balance (token_id : token_id)
                            (addr : Address)
-                           (state : State) : option N := 
-  do ledger <- FMap.find token_id state.(assets) ;
-  FMap.find addr ledger.(balances).
+                           (state : State) : N := 
+  match FMap.find token_id state.(assets) with
+  | Some ledger => with_default 0%N (FMap.find addr ledger.(balances))
+  | None => 0%N
+  end.
 
-Definition try_transfer (caller : Address)
-                        (params : transfer)
-                        (state : State)
-                        : option TokenLedger :=
+Definition get_owner_operator_tokens (owner operator : Address) 
+                                     (state : State)
+                                     : option operator_tokens := 
+  do operator_tokens <- FMap.find owner state.(operators) ;
+  FMap.find operator operator_tokens.
+
+Definition try_single_transfer (caller : Address)
+                               (params : transfer)
+                               (state : State)
+                               : option State :=
   (* do _ <- address_has_sufficient_asset_balance transfer_params.(transfer_token_id) transfer_params.(from_) transfer_params.(amount) ; *)
   do _ <- address_has_transfer_permission caller params.(from_) ;
   do ledger <- FMap.find params.(transfer_token_id) state.(assets) ;
-  do current_owner_balance <- address_balance params.(transfer_token_id) params.(from_) state ;
-  let new_balances : FMap Address N := FMap.add params.(from_) (current_owner_balance - params.(amount)) ledger.(balances) in
-  let new_balances : FMap Address N := FMap.partial_alter (fun balance => Some ((with_default 0 balance) + params.(amount))) params.(to_) new_balances in
-  Some (ledger<|balances := new_balances|>).
+  let current_owner_balance := address_balance params.(transfer_token_id) params.(from_) state in
+  let new_balances := FMap.add params.(from_) (current_owner_balance - params.(amount)) ledger.(balances) in
+  let new_balances := FMap.partial_alter (fun balance => Some ((with_default 0 balance) + params.(amount))) params.(to_) new_balances in
+  let new_ledger := ledger<|balances := new_balances|> in
+  Some (state<|assets ::= FMap.add params.(transfer_token_id) new_ledger|>).
+
+Definition transfer_check_permissions (caller : Address)
+                                      (params : transfer)
+                                      (policy : permissions_descriptor)
+                                      (state : State)
+                                      : option unit := 
+  (* if caller is owner of transfer, then check policy if self_transfer is allowed *)
+  if (address_eqb caller params.(from_))
+  then 
+    returnIf match policy.(descr_self) with
+             | self_transfer_permitted => false
+             | self_transfer_denied => true
+             end
+  else 
+    do operators_map <- FMap.find params.(from_) state.(operators) ;
+    do op_tokens <- FMap.find caller operators_map ;
+    match op_tokens with
+    | all_tokens => Some tt
+    | some_tokens token_ids => if (existsb (fun id => id =? params.(transfer_token_id)) token_ids)
+                               then Some tt
+                               else None
+    end.
+    (* check if operator has the necessary permissions *)
+
+
+Definition try_transfer (caller : Address)
+                        (transfers : list transfer)
+                        (state : State)
+                        : option TokenLedger :=
+  let check_transfer_iterator state_opt params :=
+    do state <- state_opt ;
+    do _ <- transfer_check_permissions caller params  state.(permission_policy) state;
+    try_single_transfer caller params state in   
+  (* returns the new state if all transfers *can* succeed, otherwise returns None *)
+  do state_opt <- fold_left check_transfer_iterator transfers (Some state) ;
+  (* TODO: create callback actions *)
+  None.
   
+Definition get_balance_of_callback (caller : Address)
+                                     (param : balance_of_param)
+                                     (state : State)
+                                     : ActionBody :=
+  let bal_req_iterator (bal_req : balance_of_request) :=
+    let owner_bal := address_balance bal_req.(bal_req_token_id) bal_req.(owner) state in 
+    Build_balance_of_response bal_req owner_bal in
+  let responses := map bal_req_iterator param.(bal_requests) in
+  act_call caller 0%Z (@serialize (list balance_of_response) _ responses).
+
+Definition get_total_supply_callback (caddr : Address)
+                                     (caller : Address)
+                                     (param : total_supply_param)
+                                     (state : State)
+                                     : list total_supply_response :=
+  let token_id_balance (token_id : token_id) : N :=
+    match FMap.find token_id state.(assets) with
+    | Some ledger => fold_left N.add (FMap.values ledger.(balances)) 0%N
+    | None => 0%N
+    end in
+  let mk_response (token_id : token_id) : total_supply_response := Build_total_supply_response token_id (token_id_balance token_id) in 
+  map mk_response param.(supply_param_token_ids).
+  
+
+Definition update_operators (caller : Address)
+                            (updates : list update_operator)
+                            (state : State)
+                            : State := 
+  let exec_add params (state_ : State) : State :=
+    (* only the owner of the token is allowed to update their operators *)
+    if (negb (address_eqb caller params.(op_param_owner)))
+    then state_
+    else 
+      let operator_tokens : FMap Address operator_tokens := with_default FMap.empty (FMap.find caller state_.(operators)) in
+      (* Add new operator *)
+      let operator_tokens := FMap.add params.(op_param_operator) params.(op_param_tokens) operator_tokens in
+      state_<| operators ::= FMap.add caller operator_tokens |> in
+  let exec_update state_ op := match op with
+                               | add_operator params => exec_add params state_
+                               | remove_operator params => exec_add params state_
+                               end in 
+  fold_left exec_update updates state.
+
+Definition operator_tokens_eqb (a b : operator_tokens) : bool := 
+  match (a, b) with
+  | (all_tokens, all_tokens) => true
+  | (some_tokens a', some_tokens b') => 
+    let fix my_list_eqb l1 l2 :=
+      match (l1, l2) with
+      | (x :: l1, y :: l2) => if x =? y
+                              then my_list_eqb l1 l2
+                              else false 
+      | ([], []) => true
+      | _ => false
+      end in my_list_eqb a' b'
+  | _ => false
+  end.
+
+Definition get_is_operator_response (caller : Address)
+                                    (params : is_operator_param)
+                                    (state : State)
+                                    : ActionBody := 
+  let operator_params := params.(is_operator_operator) in
+  let operator_tokens_opt := get_owner_operator_tokens operator_params.(op_param_owner) operator_params.(op_param_operator) in
+  let is_operator_result := match operator_tokens_opt state with
+                            (* check if operator_tokens from the params and from the state are equal *)
+                            | Some op_tokens => operator_tokens_eqb op_tokens operator_params.(op_param_tokens)
+                            | None => false
+                            end in
+  let response : is_operator_response := {| operator := operator_params; is_operator := is_operator_result |} in
+  act_call caller 0%Z (serialize response).
+
+Open Scope Z_scope.
+Definition receive (chain : Chain)
+						 			 (ctx : ContractCallContext)
+									 (state : State)
+									 (maybe_msg : option Msg)
+					         : option (State * list ActionBody) :=
+  let sender := ctx.(ctx_from) in
+  let caddr := ctx.(ctx_contract_address) in
+	(* let without_actions := option_map (fun new_state => (new_state, [])) in *)
+	(* Only allow calls to this contract with no payload *)
+	if ctx.(ctx_amount) >? 0
+	then None
+	else match maybe_msg with
+	| Some (msg_is_operator params) => Some (state, [get_is_operator_response sender params state]) 
+  | _ => None
+  end.  
+  
+
+Definition init (chain : Chain)
+								(ctx : ContractCallContext)
+								(setup : Setup) : option State := 
+  Some {| permission_policy := setup.(permission_policy_);
+          assets := FMap.empty;
+          operators := FMap.empty |}.
+
+Ltac solve_contract_proper :=
+  repeat
+    match goal with
+    | [|- ?x _  = ?x _] => unfold x
+    | [|- ?x _ _ = ?x _ _] => unfold x
+    | [|- ?x _ _ _ = ?x _ _ _] => unfold x
+    | [|- ?x _ _ _ _ = ?x _ _ _ _] => unfold x
+    | [|- ?x _ _ _ _ = ?x _ _ _ _] => unfold x
+    | [|- ?x _ _ _ _ _ = ?x _ _ _ _ _] => unfold x
+    | [|- Some _ = Some _] => f_equal
+    | [|- pair _ _ = pair _ _] => f_equal
+    | [|- (if ?x then _ else _) = (if ?x then _ else _)] => destruct x
+    | [|- match ?x with | _ => _ end = match ?x with | _ => _ end ] => destruct x
+    | [H: ChainEquiv _ _ |- _] => rewrite H in *
+    | _ => subst; auto
+    end.
+
+Lemma init_proper :
+  Proper (ChainEquiv ==> eq ==> eq ==> eq) init.
+Proof. repeat intro; solve_contract_proper.	Qed.
+
+Lemma receive_proper :
+  Proper (ChainEquiv ==> eq ==> eq ==> eq ==> eq) receive.
+Proof. repeat intro; solve_contract_proper. Qed.
+
+Definition contract : Contract Setup Msg State :=
+  build_contract init init_proper receive receive_proper.
+
 End FA2Token.
